@prefix eps:    <http://cltl.nl/episodicawareness/> .
@prefix gaf:    <http://groundedannotationframework.org/gaf#> .
@prefix owl:    <http://www.w3.org/2002/07/owl#> .
@prefix rdf:    <http://www.w3.org/1999/02/22-rdf-syntax-ns#> .
@prefix sem:    <http://semanticweb.cs.vu.nl/2009/11/sem/> .
@prefix xml:    <http://www.w3.org/XML/1998/namespace> .
@prefix xsd:    <http://www.w3.org/2001/XMLSchema#> .
@prefix foaf:   <http://xmlns.com/foaf/0.1/> .
@prefix prov:   <http://www.w3.org/ns/prov#> .
@prefix rdfs:   <http://www.w3.org/2000/01/rdf-schema#> .
@prefix skos:   <http://www.w3.org/2004/02/skos/core#> .
@prefix grasp:  <http://groundedannotationframework.org/grasp#> .
@prefix graspe: <http://groundedannotationframework.org/grasp/emotion#> .
@prefix graspf: <http://groundedannotationframework.org/grasp/factuality#> .
@prefix grasps: <http://groundedannotationframework.org/grasp/sentiment#> .
@base <http://www.w3.org/2002/07/owl#> .

[ rdf:type owl:Ontology
 ] .

#################################################################
#    Annotation properties
#################################################################

###  http://www.w3.org/2004/02/skos/core#broadMatch
skos:broadMatch
    rdf:type owl:AnnotationProperty .


###  http://www.w3.org/2004/02/skos/core#closeMatch
skos:closeMatch
    rdf:type owl:AnnotationProperty .


###  http://www.w3.org/2004/02/skos/core#narrowMatch
skos:narrowMatch
    rdf:type owl:AnnotationProperty .


###  http://www.w3.org/ns/prov#category
prov:category
    rdf:type owl:AnnotationProperty .


###  http://www.w3.org/ns/prov#component
prov:component
    rdf:type owl:AnnotationProperty .


###  http://www.w3.org/ns/prov#definition
prov:definition
    rdf:type owl:AnnotationProperty .


###  http://www.w3.org/ns/prov#inverse
prov:inverse
    rdf:type owl:AnnotationProperty .


###  http://www.w3.org/ns/prov#qualifiedForm
prov:qualifiedForm
    rdf:type owl:AnnotationProperty .


#################################################################
#    Object Properties
#################################################################

###  http://cltl.nl/episodicawareness/contextProperty
eps:contextProperty
    rdf:type               owl:ObjectProperty ;
    owl:equivalentProperty sem:eventProperty ;
    rdfs:comment           "Context properties connect Context to other SEM Core entities." ;
    rdfs:label             "context property" .


###  http://cltl.nl/episodicawareness/hasContext
eps:hasContext
    rdf:type           owl:ObjectProperty ;
    rdfs:subPropertyOf eps:contextProperty ;
    rdfs:domain        gaf:Instance, sem:Event ;
    rdfs:range         eps:Context .


###  http://cltl.nl/episodicawareness/hasDetection
eps:hasDetection
    rdf:type           owl:ObjectProperty ;
    rdfs:subPropertyOf eps:contextProperty ;
    rdfs:domain        eps:Context ;
    rdfs:range         grasp:Detection .


###  http://groundedannotationframework.org/gaf#containsDenotation
gaf:containsDenotation
    rdf:type      owl:ObjectProperty ;
    owl:inverseOf gaf:denotedIn ;
    rdfs:domain   gaf:Mention ;
    rdfs:range    gaf:Instance .


###  http://groundedannotationframework.org/gaf#denotedBy
gaf:denotedBy
    rdf:type           owl:ObjectProperty ;
    rdfs:subPropertyOf gaf:denotedIn ;
    owl:inverseOf      gaf:denotes ;
    rdfs:domain        gaf:Instance ;
    rdfs:range         gaf:Mention .


###  http://groundedannotationframework.org/gaf#denotedIn
gaf:denotedIn
    rdf:type    owl:ObjectProperty ;
    rdfs:domain gaf:Instance ;
    rdfs:range  gaf:Mention .


###  http://groundedannotationframework.org/gaf#denotes
gaf:denotes
    rdf:type           owl:ObjectProperty ;
    rdfs:subPropertyOf gaf:containsDenotation ;
    rdfs:domain        gaf:Mention ;
    rdfs:range         gaf:Instance .


###  http://groundedannotationframework.org/grasp#hasAttribution
grasp:hasAttribution
    rdf:type      owl:ObjectProperty ;
    owl:inverseOf grasp:isAttributionFor ;
    rdfs:domain   gaf:Mention ;
    rdfs:range    grasp:Attribution .


###  http://groundedannotationframework.org/grasp#isAttributionFor
grasp:isAttributionFor
    rdf:type    owl:ObjectProperty ;
    rdfs:domain grasp:Attribution ;
    rdfs:range  gaf:Mention .


###  http://groundedannotationframework.org/grasp#wasAttributedTo
grasp:wasAttributedTo
    rdf:type           owl:ObjectProperty ;
    rdfs:subPropertyOf prov:wasAttributedTo ;
    rdfs:domain        gaf:Mention ;
    rdfs:range         grasp:Source ;
    rdfs:comment       "States that a gaf:Mention was attributed to a gaf:Instance. This is a sub property of the prov:wasAttributedTo relation that can be used to relate any prov:Entity to any prov:Agent."^^xsd:string ;
    rdfs:label         "was attributed to" .


###  http://semanticweb.cs.vu.nl/2009/11/sem/eventProperty
sem:eventProperty
    rdf:type     owl:ObjectProperty ;
    rdfs:comment "Event properties connect Events to other SEM Core entities." ;
    rdfs:label   "event property" .


###  http://semanticweb.cs.vu.nl/2009/11/sem/hasActor
sem:hasActor
    rdf:type           owl:ObjectProperty ;
    rdfs:subPropertyOf sem:eventProperty ;
    rdfs:range         sem:Actor ;
    rdfs:comment       "Has actor is used to state which Actors or Objects participate in an Event." ;
    rdfs:label         "has Actor" .


###  http://semanticweb.cs.vu.nl/2009/11/sem/hasPlace
sem:hasPlace
    rdf:type           owl:ObjectProperty ;
    rdfs:subPropertyOf sem:eventProperty ;
    rdfs:range         sem:Place ;
    rdfs:comment       "Has place is used to state in which Place(s) an Event happened. Coordinates can be attached to the Place with the W3C Geospatial Vocabulary (http://www.w3.org/2005/Incubator/geo/XGR-geo-20071023/)." ;
    rdfs:label         "has Place" .


###  http://semanticweb.cs.vu.nl/2009/11/sem/hasSubEvent
sem:hasSubEvent
    rdf:type           owl:ObjectProperty ;
    rdfs:subPropertyOf sem:eventProperty ;
    owl:inverseOf      sem:subEventOf ;
    rdfs:domain        sem:Event ;
    rdfs:range         sem:Event ;
    rdfs:comment       "Has subevent connects an Event to other Events that belong to it. This is a very generic property that does not mean the subevents fully define the superconcept or that there is any causal relationship." ;
    rdfs:label         "has subevent" .


###  http://semanticweb.cs.vu.nl/2009/11/sem/hasTime
sem:hasTime
    rdf:type           owl:ObjectProperty ;
    rdfs:subPropertyOf sem:eventProperty ;
    rdfs:range         sem:Time ;
    rdfs:comment       "Has time is used to indicate at which time an Event took place or when a property under the Temporary Constraint is valid. Has time points to a symbolic representation of time, which allows semantic relations between time resources. (see http://www.w3.org/TR/owl-time/)" ;
    rdfs:label         "has Time" .


###  http://semanticweb.cs.vu.nl/2009/11/sem/subEventOf
sem:subEventOf
    rdf:type     owl:ObjectProperty ;
    rdfs:comment "Inverse property of hasSubEvent" ;
    rdfs:label   "subevent of" .


###  http://www.w3.org/1999/02/22-rdf-syntax-ns#value
rdf:value
    rdf:type owl:ObjectProperty .


###  http://www.w3.org/ns/prov#hadDerivation
prov:hadDerivation
    rdf:type      owl:ObjectProperty ;
    owl:inverseOf prov:wasDerivedFrom .


###  http://www.w3.org/ns/prov#wasAttributedTo
prov:wasAttributedTo
    rdf:type owl:ObjectProperty .


###  http://www.w3.org/ns/prov#wasDerivedFrom
prov:wasDerivedFrom
    rdf:type           owl:ObjectProperty ;
    rdfs:subPropertyOf owl:topObjectProperty ;
    rdfs:domain        gaf:Mention ;
    rdfs:range         grasp:Detection, grasp:Utterance ;
    rdfs:comment       "The more specific subproperties of prov:wasDerivedFrom (i.e., prov:wasQuotedFrom, prov:wasRevisionOf, prov:hadPrimarySource) should be used when applicable."@en ;
    rdfs:label         "wasDerivedFrom" ;
    prov:category      "starting-point" ;
    prov:component     "derivations" ;
    prov:definition    "A derivation is a transformation of an entity into another, an update of an entity resulting in a new one, or the construction of a new entity based on a pre-existing entity."@en ;
    prov:inverse       "hadDerivation" ;
    prov:qualifiedForm prov:Derivation .


#################################################################
#    Data properties
#################################################################

###  http://semanticweb.cs.vu.nl/2009/11/sem/hasBeginTimeStamp
sem:hasBeginTimeStamp
    rdf:type           owl:DatatypeProperty ;
    rdfs:subPropertyOf sem:hasTimeStamp ;
    rdfs:comment       "Has begin timestamp is used to indicate the beginning of a time interval. Omitting the hasBeginTimeStamp while stating a hasEndTimeStamp is interpreted as an open ended interval." ;
    rdfs:label         "has begin timestamp" .


###  http://semanticweb.cs.vu.nl/2009/11/sem/hasTimeStamp
sem:hasTimeStamp
    rdf:type owl:DatatypeProperty .


#################################################################
#    Classes
#################################################################

###  http://cltl.nl/episodicawareness/Context
eps:Context
    rdf:type owl:Class .


###  http://groundedannotationframework.org/gaf#Assertion
gaf:Assertion
    rdf:type        owl:Class ;
    rdfs:subClassOf gaf:Instance .


###  http://groundedannotationframework.org/gaf#Instance
gaf:Instance
    rdf:type            owl:Class ;
    owl:equivalentClass [ rdf:type           owl:Restriction ;
                          owl:onProperty     gaf:denotedBy ;
                          owl:someValuesFrom gaf:Mention ] ;
    rdfs:subClassOf     owl:Thing ;
    owl:disjointWith    grasp:AttributionValue ;
    rdfs:comment        "Instances are statements about real world entities, including actions, processes and abstract notions. They are the primary subject of individuals of type gaf:Mention that can denote them."^^xsd:string ;
    rdfs:label          "Instance" .


###  http://groundedannotationframework.org/gaf#Mention
gaf:Mention
    rdf:type            owl:Class ;
    owl:equivalentClass [ rdf:type           owl:Restriction ;
                          owl:onProperty     gaf:denotes ;
                          owl:someValuesFrom gaf:Instance ] ;
    rdfs:subClassOf     owl:Thing ;
    owl:disjointWith    grasp:AttributionValue ;
    rdfs:comment        """Mentions are references to members of the gaf:Instance class as they occur in (web) media such as texts, video, audio, images, etc. Mentions denote gaf:Instances.

A Mention uniquely identifies the (part of a) web source that denotes the mention. We refer to the standard use of fragment identifiers for different media types. """^^xsd:string ;
    rdfs:label          "Mention" .


###  http://groundedannotationframework.org/grasp#Attribution
grasp:Attribution
    rdf:type            owl:Class ;
    owl:equivalentClass [ owl:intersectionOf ( [ rdf:type           owl:Restriction ;
                                                 owl:onProperty     grasp:isAttributionFor ;
                                                 owl:someValuesFrom gaf:Mention ]
                                               [ rdf:type           owl:Restriction ;
                                                 owl:onProperty     rdf:value ;
                                                 owl:someValuesFrom grasp:AttributionValue ] ) ;
                          rdf:type           owl:Class ] ;
    owl:disjointWith    grasp:AttributionValue ;
    rdfs:comment        "A grasp:Attribution reflects the attribution of some interpretation, some perspective to a gaf:Mention. An attribution expresses such things as certainty, emotion, polarity, sentiment, temporality."^^xsd:string ;
    rdfs:label          "Attribution" .


###  http://groundedannotationframework.org/grasp#AttributionValue
grasp:AttributionValue
    rdf:type        owl:Class ;
    rdfs:subClassOf owl:Thing ;
    rdfs:comment    "The value of a grasp:Attribution"^^xsd:string ;
    rdfs:label      "Attribution value"^^xsd:string .


###  http://groundedannotationframework.org/grasp#CertaintyValue
grasp:CertaintyValue
    rdf:type            owl:Class ;
    owl:equivalentClass [ rdf:type  owl:Class ;
                          owl:oneOf ( graspf:certain
                                      graspf:possible
                                      graspf:probable
                                      graspf:underspecified ) ] ;
    rdfs:subClassOf     grasp:FactualityValue ;
    owl:disjointWith    grasp:PolarityValue, grasp:TemporalValue ;
    rdfs:comment        "The level of certainty of a gaf:Mention"^^xsd:string ;
    rdfs:label          "Certainty Value" .


###  http://groundedannotationframework.org/grasp#Chat
grasp:Chat
    rdf:type        owl:Class ;
    rdfs:subClassOf sem:Event .


###  http://groundedannotationframework.org/grasp#Detection
grasp:Detection
    rdf:type        owl:Class ;
    rdfs:subClassOf sem:Event .


###  http://groundedannotationframework.org/grasp#EmotionValue
grasp:EmotionValue
    rdf:type            owl:Class ;
    owl:equivalentClass [ rdf:type  owl:Class ;
                          owl:oneOf ( graspe:anger
                                      graspe:disgust
                                      graspe:fear
                                      graspe:happiness
                                      graspe:sadness
                                      graspe:surprise ) ] ;
    rdfs:subClassOf     grasp:AttributionValue ;
    owl:disjointWith    grasp:FactualityValue, grasp:SentimentValue ;
    rdfs:comment        "The emotion expressed in a gaf:Mention"^^xsd:string ;
    rdfs:label          "Emotion Value" .


###  http://groundedannotationframework.org/grasp#Experience
grasp:Experience
    rdf:type        owl:Class ;
    rdfs:subClassOf gaf:Mention, sem:Event .


###  http://groundedannotationframework.org/grasp#FactualityValue
grasp:FactualityValue
    rdf:type         owl:Class ;
    rdfs:subClassOf  grasp:AttributionValue ;
    owl:disjointWith grasp:SentimentValue ;
    rdfs:label       "Factuality value"^^xsd:string .


###  http://groundedannotationframework.org/grasp#PolarityValue
grasp:PolarityValue
    rdf:type            owl:Class ;
    owl:equivalentClass [ rdf:type  owl:Class ;
                          owl:oneOf ( graspf:negative
                                      graspf:positive ) ] ;
    rdfs:subClassOf     grasp:FactualityValue ;
    owl:disjointWith    grasp:TemporalValue ;
    rdfs:comment        "The polarity of a gaf:Mention (e.g. if something is or isn't the case)"^^xsd:string ;
    rdfs:label          "Polarity Value" .


###  http://groundedannotationframework.org/grasp#SentimentValue
grasp:SentimentValue
    rdf:type            owl:Class ;
    owl:equivalentClass [ rdf:type  owl:Class ;
                          owl:oneOf ( grasps:negative
                                      grasps:positive ) ] ;
    rdfs:subClassOf     grasp:AttributionValue ;
    rdfs:comment        "The sentiment expressed by a gaf:Mention"^^xsd:string ;
    rdfs:label          "Sentiment Value" .


###  http://groundedannotationframework.org/grasp#Source
grasp:Source
    rdf:type        owl:Class ;
    rdfs:subClassOf owl:Thing ;
    rdfs:comment    "" ;
    rdfs:label      "Source" .


###  http://groundedannotationframework.org/grasp#Statement
grasp:Statement
    rdf:type        owl:Class ;
    rdfs:subClassOf gaf:Mention, sem:Event .


###  http://groundedannotationframework.org/grasp#TemporalValue
grasp:TemporalValue
    rdf:type            owl:Class ;
    owl:equivalentClass [ rdf:type  owl:Class ;
                          owl:oneOf ( graspf:future
                                      graspf:non-future ) ] ;
    rdfs:subClassOf     grasp:FactualityValue ;
    rdfs:comment        "The temporal property of a gaf:Mention"^^xsd:string ;
    rdfs:label          "Temporal Value" .


###  http://groundedannotationframework.org/grasp#Utterance
grasp:Utterance
    rdf:type        owl:Class ;
    rdfs:subClassOf sem:Event .


###  http://groundedannotationframework.org/grasp#Visual
grasp:Visual
    rdf:type        owl:Class ;
    rdfs:subClassOf sem:Event .


###  http://schema.org/Place
<http://schema.org/Place>
    rdf:type owl:Class .


###  http://semanticweb.cs.vu.nl/2009/11/sem/Actor
sem:Actor
    rdf:type        owl:Class ;
    rdfs:comment    """Actors are entities that take part in an Event, either actively or passively. Actors do not necessarily have to be sentient. They can also be objects. Actors are a thing, animate or inanimate, physical or non-physical.
""" ;
    rdfs:label      "Actor" ;
    skos:broadMatch <http://sw.opencyc.org/2009/04/07/concept/en/SomethingExisting>,
                    <http://www.loa-cnr.it/ontologies/DOLCE-Lite.owl#endurant> ;
    skos:closeMatch <http://purl.org/dc/terms/Agent>, <http://purl.org/dc/terms/AgentClass>,
                    <http://sw.opencyc.org/2009/04/07/concept/en/Agent-Generic>,
                    <http://www.ontologyportal.org/translations/SUMO.owl.txt#Agent>,
                    <http://www8.informatik.uni-erlangen.de/IMMD8/Services/cidoc-crm/erlangen-crm_090330_5_0_1.owl#E39.Actor>,
                    foaf:Agent .


###  http://semanticweb.cs.vu.nl/2009/11/sem/Event
sem:Event
    rdf:type        owl:Class ;
    rdfs:comment    "Events are things that happen. This comprises everything from historical events to web site sessions and mythical journeys. Event is the central class of SEM." ;
    rdfs:label      "Event" ;
    skos:broadMatch <http://linkedevents.org/ontology/Event>, <http://purl.org/NET/c4dm/event.owl#Event> ;
    skos:closeMatch <http://purl.org/dc/dcmitype/Event>, <http://sw.opencyc.org/2009/04/07/concept/en/Situation>,
                    <http://www.loa-cnr.it/ontologies/DOLCE-Lite.owl#perdurant>,
                    <http://www.ontologyportal.org/translations/SUMO.owl.txt#Process>,
                    <http://www8.informatik.uni-erlangen.de/IMMD8/Services/cidoc-crm/erlangen-crm_090330_5_0_1.owl#E5.Event> .


###  http://semanticweb.cs.vu.nl/2009/11/sem/Place
sem:Place
    rdf:type         owl:Class ;
    rdfs:comment     "Places are locations where an Event happens. They do not need to be physical places and hence do not necessarily need coordinates. Neither do they need to have any significance apart from them being the location of an Event." ;
    rdfs:label       "Place" ;
    skos:closeMatch  <http://purl.org/dc/terms/Location>,
                     <http://sw.opencyc.org/2009/04/07/concept/en/EnduringThing-Localized>,
                     <http://www.ontologyportal.org/translations/SUMO.owl.txt#GeographicArea>,
                     <http://www8.informatik.uni-erlangen.de/IMMD8/Services/cidoc-crm/erlangen-crm_090330_5_0_1.owl#E53.Place> ;
    skos:narrowMatch <http://www.loa-cnr.it/ontologies/DOLCE-Lite.owl#PhysicalRegion>,
                     <http://www.w3.org/2003/01/geo/wgs84_pos#SpatialThing> .


###  http://semanticweb.cs.vu.nl/2009/11/sem/Time
sem:Time
    rdf:type        owl:Class ;
    rdfs:comment    "Time contains symbolic representations of when an Event took place. Time instances do not necessarily need to have a timestamp associated with them. The Time class exists to represent semantics of time, e.g. that one thing happens before another, even though the exact timestamps are unknown." ;
    rdfs:label      "Time" ;
    skos:broadMatch <http://www.w3.org/2006/timeTemporalEntity> .


###  http://xmlns.com/foaf/0.1/Agent
foaf:Agent
    rdf:type owl:Class .


#################################################################
#    Individuals
#################################################################

###  http://groundedannotationframework.org/grasp/emotion#anger
graspe:anger
    rdf:type owl:NamedIndividual, grasp:EmotionValue .


###  http://groundedannotationframework.org/grasp/emotion#disgust
graspe:disgust
    rdf:type owl:NamedIndividual, grasp:EmotionValue .


###  http://groundedannotationframework.org/grasp/emotion#fear
graspe:fear
    rdf:type owl:NamedIndividual, grasp:EmotionValue .


###  http://groundedannotationframework.org/grasp/emotion#happiness
graspe:happiness
    rdf:type owl:NamedIndividual, grasp:EmotionValue .


###  http://groundedannotationframework.org/grasp/emotion#sadness
graspe:sadness
    rdf:type owl:NamedIndividual, grasp:EmotionValue .


###  http://groundedannotationframework.org/grasp/emotion#surprise
graspe:surprise
    rdf:type owl:NamedIndividual, grasp:EmotionValue .


###  http://groundedannotationframework.org/grasp/factuality#certain
graspf:certain
    rdf:type owl:NamedIndividual, grasp:CertaintyValue .


###  http://groundedannotationframework.org/grasp/factuality#future
graspf:future
    rdf:type owl:NamedIndividual, grasp:TemporalValue .


###  http://groundedannotationframework.org/grasp/factuality#negative
graspf:negative
    rdf:type owl:NamedIndividual, grasp:PolarityValue .


###  http://groundedannotationframework.org/grasp/factuality#non-future
graspf:non-future
    rdf:type owl:NamedIndividual, grasp:TemporalValue .


###  http://groundedannotationframework.org/grasp/factuality#positive
graspf:positive
    rdf:type owl:NamedIndividual, grasp:PolarityValue .


###  http://groundedannotationframework.org/grasp/factuality#possible
graspf:possible
    rdf:type owl:NamedIndividual, grasp:CertaintyValue .


###  http://groundedannotationframework.org/grasp/factuality#probable
graspf:probable
    rdf:type owl:NamedIndividual, grasp:CertaintyValue .


###  http://groundedannotationframework.org/grasp/factuality#underspecified
graspf:underspecified
    rdf:type owl:NamedIndividual, grasp:CertaintyValue .


###  http://groundedannotationframework.org/grasp/sentiment#negative
grasps:negative
    rdf:type owl:NamedIndividual, grasp:SentimentValue .


###  http://groundedannotationframework.org/grasp/sentiment#positive
grasps:positive
    rdf:type owl:NamedIndividual, grasp:SentimentValue .


###  Generated by the OWL API (version 4.5.9.2019-02-01T07:24:44Z) https://github.com/owlcs/owlapi
